

# MIT 18.02SC Problem Set 9

Nilangshu Sarkar

December 2025

## Part 2

### Problem 1

**Problem 1** (4: 2,2)

$$\mathbf{F}(x, y) = (y^3 - 6y) \mathbf{i} + (6x - x^3) \mathbf{j}.$$

a) Using Green's Theorem, find the simple closed curve  $C$  for which the integral

$\oint_C \mathbf{F} \cdot d\mathbf{r}$  (with positive orientation) will have the largest positive value.

b) Compute this largest positive value.

### Solution :-

a.

$$\begin{aligned} F &= (y^3 - 6y)\hat{i} + (6x - x^3)\hat{j} \\ \nabla \times F &= \frac{\partial}{\partial x}(6x - x^3) - \frac{\partial}{\partial y}(y^3 - 6y) = -3(x^2 + y^2 - 4) \\ \oint_C F \cdot d\mathbf{r} &= \iint_R (\nabla \times F) dA = \iint_R -3(x^2 + y^2 - 4) dx dy \end{aligned}$$

Now in order to search for a Curve  $C$  for the Integral  $\oint_C F \cdot d\mathbf{r}$  to be maximum, we need to find the Region  $R$  where the Double Integral  $\iint_R -3(x^2 + y^2 - 4) dx dy$  is maximum.

Note that the value of  $-3(x^2 + y^2 - 4)$  Decreases with Increase of both  $x$  and  $y$ .

So, we can set our region to be the one where  $-3(x^2 + y^2 - 4)$  is positive. This gives us

$$-3(x^2 + y^2 - 4) \geq 0 \implies x^2 + y^2 \leq 2^2 \text{ ...this gives our required } R$$

The  $C$  bounding this  $R$  is the

$$\text{Circle } x^2 + y^2 = 2^2$$

**b.**

Converting to Polar Coordinate, we get

$$\iint_{x^2+y^2 \leq 2^2} -3(x^2+y^2-4)dxdy = \int_{\theta=0}^{2\pi} \int_{r=0}^2 -3\left((r \cos(\theta))^2 + (r \sin(\theta))^2 - 4\right) r dr d\theta$$

Hence our Integral computes out to be

$$\begin{aligned} & \int_{\theta=0}^{2\pi} \int_{r=0}^2 -3\left((r \cos(\theta))^2 + (r \sin(\theta))^2 - 4\right) r dr d\theta \\ &= \int_{\theta=0}^{2\pi} \int_{r=0}^2 -3\left(r^3 - 4r\right) dr d\theta = 24\pi \end{aligned}$$

Therefore, the **Largest Positive Value is  $24\pi$**

## Problem 2

### Problem 2 (6: 2,2,2)

In the reading V4.2 (pp.1-3) it is shown that in the context of 2D fluid flows, Green's theorem in normal form combined with the principle of conservation of mass imply that  $\text{div}(\mathbf{F})$ , the divergence of the flow field  $\mathbf{F}(x, y)$ , represents the (signed) rate of mass per unit time per unit area which originates at the point  $(x, y)$ , or the source or sink rate for short. This extends to non-steady flows  $\mathbf{F}(x, y, t)$ , and leads directly to the *Equation of Continuity* for fluid flows, which is the statement of conservation of mass and hence one of the basic physical principles of fluid dynamics. We'll continue to use  $\rho$  for the density (instead of  $\delta$  used in the Notes).

The divergence of a vector field  $\mathbf{F}(x, y, t)$  in this context is defined with respect to the space variables only, that is, if  $\mathbf{F}(x, y, t) = \langle M(x, y, t), N(x, y, t) \rangle$  is a smooth vector field, then  $\text{div}(\mathbf{F}) = \frac{\partial M}{\partial x} + \frac{\partial N}{\partial y}$ .

Then for the case of a flow field  $\mathbf{F}(x, y, t) = \rho(x, y, t) \mathbf{v}(x, y, t)$  with density  $\rho(x, y, t)$  and velocity  $\mathbf{v}(x, y, t)$ , the equation of continuity reads

$$\frac{\partial \rho}{\partial t} + \text{div}(\mathbf{F}) = 0.$$

Note that for *steady* flows, which by definition means  $\rho = \rho(x, y)$  and  $\mathbf{v} = \mathbf{v}(x, y)$ , the equation of continuity holds if and only if  $\text{div}(\mathbf{F}) = 0$ . Thus conservation of mass for steady flows is equivalent to the absence of any sources or sinks, which makes sense.

a) For non-steady flows, assuming that the physical interpretation of  $\text{div}(\mathbf{F})$  is the same as in the case of steady flows (at each time  $t$ ), explain why the equation of continuity is in fact the statement of conservation of mass.

*Hint:* take an arbitrary bounded region  $\mathcal{R}$  and integrate both terms of the continuity equation over  $\mathcal{R}$ . Then use Green's theorem in normal form.

b) Let  $g(x, y, t)$  be a smooth scalar function, and again define the gradient of  $g(x, y, t)$  in this case to be with respect to just the space variables:  $\nabla g = \langle g_x, g_y \rangle$ . Then if and  $\mathbf{G}(x, y, t) = \langle M(x, y, t), N(x, y, t) \rangle$  is a smooth vector field, use the product rule to show that

$$\text{div}(g \mathbf{G}) = g \text{div}(\mathbf{G}) + \mathbf{G} \cdot \nabla g$$

c) Refer to the definition of the convective derivative  $\frac{Df}{Dt}$  given in p-set 5 #2, and the definition of incompressibility for flows  $\frac{D\rho}{Dt} = 0$ , as given in p-set 5 #3.

Combining: the equation of continuity; the result of part(b) above; and the result of p-set 5 #2, show that the flow  $\mathbf{F}(x, y, t) = \rho(x, y, t) \mathbf{v}(x, y, t)$  is incompressible if and only if

$$\text{div}(\mathbf{v}) = 0.$$

This is thus an equivalent condition for the incompressibility of a flow.

### Solution :-

a.

Equation of Continuity :-

$$\frac{\partial \rho}{\partial t} + \nabla \cdot (F) = 0$$

$$\Rightarrow \iint_R \frac{\partial \rho}{\partial t} dA + \iint_R \nabla \cdot (F) dA = \iint_R 0 dA = 0 \text{ [Taking Double Integral on both Sides]}$$

$$\begin{aligned} \Rightarrow \frac{\partial}{\partial t} \iint_R (\rho) dA + \oint_C F \cdot \hat{n} ds &= 0 \text{ [By Green's Theorem (Normal Form), } \oint_C F \cdot \hat{n} ds = \iint_R \nabla \cdot (F) dA] \\ \Rightarrow \frac{\partial M}{\partial t} + \oint_C F \cdot \hat{n} ds &= 0 \text{ [Since } \iint_R (\rho) dA = M] \end{aligned}$$

Note:-

•

$$\frac{\partial M}{\partial t}$$

denotes the Mass Increment with respect to Time at each Position.

•

$$\oint_C F \cdot \hat{n} ds$$

denotes the Flux of Flow at each position i.e. positive outward.

• Sum of these two factors equals Zero implies that Mass is Conserved.

Hence proved that the **Equation of Continuity implies Law of Conservation of Mass**.

b.

$$\begin{aligned} \nabla \cdot (gG) &= \nabla \cdot (gM + gN) = \frac{\partial}{\partial x}(gM) + \frac{\partial}{\partial y}(gN) \\ &= g_x M + g M_x + g_y N + g N_y = g(M_x + N_y) + (g_x M + g_y N) \\ &= g(M_x + N_y) + \nabla(g) \cdot \langle M, N \rangle = g \nabla \cdot (G) + \nabla(g) \cdot (G) \end{aligned}$$

Hence proved,

$$\nabla \cdot (gG) = g \nabla \cdot (G) + \nabla(g) \cdot (G)$$

c.

The Expression obtained in p-set 5

$$\frac{Df}{Dt} = \frac{\partial f}{\partial t} + v \cdot \nabla f$$

$$\begin{aligned} \Rightarrow \frac{D\rho}{Dt} &= \frac{\partial \rho}{\partial t} + v \cdot \nabla \rho = -\nabla \cdot (F) + v \cdot \nabla(\rho) \text{ [By Equation of Continuity]} \\ &= -\nabla \cdot (\rho v) + v \cdot \nabla(\rho) \text{ [Given } F = \rho v] \\ &= -\rho \nabla \cdot (v) - \nabla(\rho) \cdot (v) + v \cdot \nabla(\rho) \text{ [From result of part b.]} \\ &= -\rho \nabla \cdot (v) \end{aligned}$$

Therefore,

$$\frac{D\rho}{Dt} = 0 \implies -\rho \nabla \cdot (v) = 0$$

Hence proved that for a Fluid to be incompressible

$$\nabla \cdot (v) = 0$$